\documentclass[h]{article}
\usepackage[margin=0.5in]{geometry}
\usepackage{amsfonts}
\title{CS 2050 Homework 2}
\date{January 22nd, 2014}
\author{Hemen Shah \\ Section B1 \\ Grading TA: Akshay}


\begin{document}

\maketitle

\section*{1.2 \#20}

A says The two of us are both knights.\newline
B says A is a knave.\newline
p: A is knight\newline 
q: B is a knight\newline
\begin{tabular}{|c c|}\hline
(p $\rightarrow$ (p $\wedge$ q)) $\wedge$ ($\neg$p $\rightarrow$ $\neg$(p $\wedge$ q)) $\wedge$ (q $\rightarrow$ $\neg$p) $\wedge$ ($\neg$q $\rightarrow$ $\neg \neg$p) & given\\ 
(p $\rightarrow$ (p $\wedge$ q)) $\wedge$ ($\neg$p $\rightarrow$ ($\neg$p $\vee$ $\neg$q)) $\wedge$ (q $\rightarrow$ $\neg$p) $\wedge$ ($\neg$q $\rightarrow$ $\neg \neg$p) & demorgans \\ 
(p $\rightarrow$ (p $\wedge$ q)) $\wedge$ ($\neg$p $\rightarrow$ ($\neg$p $\vee$ $\neg$q)) $\wedge$ (q $\rightarrow$ $\neg$p) $\wedge$ ($\neg$q $\rightarrow$ p) & double negation\\ 
($\neg$p $\vee$ (p $\wedge$ q)) $\wedge$ ($\neg$p $\rightarrow$ ($\neg$p $\vee$ $\neg$q)) $\wedge$ (q $\rightarrow$ $\neg$p) $\wedge$ ($\neg$q $\rightarrow$ p) & material implication\\ 
($\neg$p $\vee$ (p $\wedge$ q)) $\wedge$ ($\neg \neg$p $\vee$ ($\neg$p $\vee$ $\neg$q)) $\wedge$ (q $\rightarrow$ $\neg$p) $\wedge$ ($\neg$q $\rightarrow$ p) & material implication\\ 
($\neg$p $\vee$ (p $\wedge$ q)) $\wedge$ (p $\vee$ ($\neg$p $\vee$ $\neg$q)) $\wedge$ (q $\rightarrow$ $\neg$p) $\wedge$ ($\neg$q $\rightarrow$ p) & double negation\\ 
($\neg$p $\vee$ (p $\wedge$ q)) $\wedge$ (p $\vee$ ($\neg$p $\vee$ $\neg$q)) $\wedge$ ($\neg $q $\vee$ $\neg$p) $\wedge$ ($\neg$q $\rightarrow$ p) & material implication\\ 
($\neg$p $\vee$ (p $\wedge$ q)) $\wedge$ (p $\vee$ ($\neg$p $\vee$ $\neg$q)) $\wedge$ ($\neg $q $\vee$ $\neg$p) $\wedge$ ($\neg \neg$q $\vee$ p) & material implication\\ 
($\neg$p $\vee$ (p $\wedge$ q)) $\wedge$ (p $\vee$ ($\neg$p $\vee$ $\neg$q)) $\wedge$ ($\neg $q $\vee$ $\neg$p) $\wedge$ (q $\vee$ p) & double negation\\
($\neg$p $\vee$ (p $\wedge$ q)) $\wedge$ ((p $\vee$ $\neg$p) $\vee$ $\neg$q) $\wedge$ ($\neg $q $\vee$ $\neg$p) $\wedge$ (q $\vee$ p) & associative \\ 
($\neg$p $\vee$ (p $\wedge$ q)) $\wedge$ (T $\vee$ $\neg$q) $\wedge$ ($\neg $q $\vee$ $\neg$p) $\wedge$ (q $\vee$ p) & negation law \\ 
($\neg$p $\vee$ (p $\wedge$ q)) $\wedge$ (T) $\wedge$ ($\neg $q $\vee$ $\neg$p) $\wedge$ (q $\vee$ p) & domination \\ 
($\neg$p $\vee$ (p $\wedge$ q)) $\wedge$ ($\neg $q $\vee$ $\neg$p) $\wedge$ (q $\vee$ p) & identity \\ 
(($\neg$p $\vee$ p)$\wedge$ ($\neg$p $\vee$ q)) $\wedge$ ($\neg $q $\vee$ $\neg$p) $\wedge$ (q $\vee$ p) & distributive \\
((p $\vee$ $\neg$p)$\wedge$ ($\neg$p $\vee$ q)) $\wedge$ ($\neg $q $\vee$ $\neg$p) $\wedge$ (q $\vee$ p) & commutative \\
((T)$\wedge$ ($\neg$p $\vee$ q)) $\wedge$ ($\neg $q $\vee$ $\neg$p) $\wedge$ (q $\vee$ p) & domination \\
(($\neg$p $\vee$ q)$\wedge$ (T)) $\wedge$ ($\neg $q $\vee$ $\neg$p) $\wedge$ (q $\vee$ p) & commutative \\
($\neg$p $\vee$ q) $\wedge$ ($\neg $q $\vee$ $\neg$p) $\wedge$ (q $\vee$ p) & identity \\
($\neg$p $\vee$ q) $\wedge$ ($\neg $p $\vee$ $\neg$q) $\wedge$ (q $\vee$ p) & commutiative \\
($\neg$p $\wedge$ (q $\vee$ $\neg$q)) $\wedge$ (q $\vee$ p) & distributive \\
($\neg$p $\wedge$ T) $\wedge$ (q $\vee$ p) & negation law \\
$\neg$p $\wedge$ (q $\vee$ p) & identity  \\
($\neg$p $\wedge$ q) $\vee$($\neg$p $\wedge$p) & distributive  \\
($\neg$p $\wedge$ q) $\vee$(p $\wedge$ $\neg$p) & commutative  \\
($\neg$p $\wedge$ q) $\vee$ F & negation law  \\
$\neg$p $\wedge$ q & identity  \\ \hline
\end{tabular}\newline \newline
LADBAP - A is knave B is knight

\section*{1.2 \#22}
A says A is a knight \newline
B says B is a knight \newline
p: A is a knight \newline
q: B is a knight \newline
\begin{tabular}{|c c|} \hline
$(p \rightarrow p) \wedge (\neg p \rightarrow \neg p) \wedge (q \rightarrow q) \wedge (\neg q \rightarrow \neg q)$ & given\\
$(\neg p \vee p) \wedge (\neg p \rightarrow \neg p) \wedge (q \rightarrow q) \wedge (\neg q \rightarrow \neg q)$ & material implication\\
$(\neg p \vee p) \wedge (\neg \neg p \vee \neg p) \wedge (q \rightarrow q) \wedge (\neg q \rightarrow \neg q)$ & material implication\\
$(\neg p \vee p) \wedge (\neg \neg p \vee \neg p) \wedge (\neg q \vee q) \wedge (\neg q \rightarrow \neg q)$ & material implication\\
$(\neg p \vee p) \wedge (\neg \neg p \vee \neg p) \wedge (\neg q \vee q) \wedge (\neg \neg q \vee \neg q)$ & material implication\\
$(\neg p \vee p) \wedge ( p \vee \neg p) \wedge (\neg q \vee q) \wedge (\neg \neg q \vee \neg q)$ & double negation\\
$(\neg p \vee p) \wedge ( p \vee \neg p) \wedge (\neg q \vee q) \wedge (q \vee \neg q)$ & double negation\\
$( p \vee \neg p) \wedge ( p \vee \neg p) \wedge (\neg q \vee q) \wedge (q \vee \neg q)$ & commutative\\
$( p \vee \neg p) \wedge ( p \vee \neg p) \wedge (q \vee \neg q) \wedge (q \vee \neg q)$ & commutative\\
$T \wedge ( p \vee \neg p) \wedge (q \vee \neg q) \wedge (q \vee \neg q)$ & negation law\\
$T \wedge T \wedge (q \vee \neg q) \wedge (q \vee \neg q)$ & negation law\\
$T \wedge T \wedge T \wedge (q \vee \neg q)$ & negation law\\
$T \wedge T \wedge T \wedge T$ & negation law\\
$T \wedge T \wedge T$ & idempotent\\
$T \wedge T$ & idempotent\\
$T$ & idempotent\\ \hline
\end{tabular} \newline \newline
LADBAP - We don't know anything about either of them. Their being a knight or a knave does not change the truth value

\section*{1.3 \#4}
a.\newline
\begin{tabular}{|c|c|c|c|c|c|c|} \hline
p & q & r & (p $\vee$ q) &(p $\vee$ q) $\vee$ r& (q $\vee$ r) & p $\vee$ (q $\vee$ r)\\ \hline
T & T & T & T & T & T & T\\ \hline
T & T & F & T & T & T & T\\ \hline
T & F & T & T & T & T & T\\ \hline
T & F & F & T & T & F & T\\ \hline
F & T & T & T & T & T & T\\ \hline
F & T & F & T & T & T & T\\ \hline
F & F & T & F & T & T & T\\ \hline
F & F & F & F & F & F & F\\ \hline

\end{tabular}\newline \newline
The columns for $(p \vee q) \vee r$ and $p \vee (q \vee r)$ match exactly and so are equivalent

\section*{1.3 \#8}
a. Kwame will take a job in industry or go to graduate school\newline
i: Kwame will take a job in industry \newline
g: Kwame will go to graduate school\newline
$\neg(i \vee g) \newline
\neg i \wedge \neg g $ \newline
Kwame will not take a job in industry and he will not go to graduate school
\newline \newline
b. Yoshiko knows Java and calculus\newline
j: Yoshiko knows Java\newline 
c: Yoshiko knows calculus\newline
$\neg (j \wedge c) \newline
\neg j \vee \neg c \newline$
Yoshiko does not know either Java or calculus or both.
\newline \newline
c. James is young and strong\newline
y: James is young \newline
s: James is strong \newline
$ \neg (y \wedge s)\newline
\neg y \vee \neg s \newline$
James is not young or not strong or not both
\newline \newline
d. Rita will move to Oregon or Washington\newline
o: Rita will move to Oregon \newline
w: Rita will move to Washington\newline
$ \neg (o \vee w)\newline
\neg o \wedge \neg w \newline $
Rita will not move to Oregon and Washington

\section*{1.3 \#10}
Tautology by truth tables\newline
$[p \wedge (p \rightarrow q)] \rightarrow q $\newline
\begin{tabular}{|c|c|c|c|c|}\hline
p & q & $p \rightarrow q$ & $p \wedge (p \rightarrow q)$ & $[p \wedge (p \rightarrow q)] \rightarrow q $\\ \hline
T & T & T & T & T\\ \hline
T & F & F & F & T\\ \hline
F & T & T & T & T\\ \hline
F & F & T & T & T\\ \hline
\end{tabular}
\newline \newline
$[(p \vee q) \wedge (p \rightarrow r) \wedge (q \rightarrow r)] \rightarrow r$\newline
\begin{tabular}{|c|c|c|c|c|c|c|c|c|} \hline
p & q & r & $(p \vee q)$ & $(p \rightarrow r)$ & $(q \rightarrow r)$ & $(p \vee q) \wedge (p \rightarrow r)$ & $(p \vee q) \wedge (p \rightarrow r) \wedge (q \rightarrow r)$ & $[(p \vee q) \wedge (p \rightarrow r) \wedge (q \rightarrow r)] \rightarrow r$ \\ \hline
T & T & T & T & T & T & T & T & T\\ \hline
T & T & F & T & F & F & F & F & T\\ \hline
T & F & T & T & T & T & T & T & T\\ \hline
T & F & F & T & F & T & F & F & T\\ \hline
F & T & T & T & T & T & T & T & T\\ \hline
F & T & F & T & T & F & T & F & T\\ \hline
F & F & T & F & T & T & F & F & T\\ \hline
F & F & F & F & T & T & F & F & T\\ \hline
\end{tabular}

\section*{1.3 \#12}
Prove tautology by logical equivalence\newline
$[p \wedge (p \rightarrow q)] \rightarrow q $\newline
\begin{tabular}{|c c|}\hline
$[p \wedge (p \rightarrow q)] \rightarrow q $ & given \\ 
$[p \wedge (\neg p \vee q)] \rightarrow q $ & material implication \\
$\neg [p \wedge (\neg p \vee q)] \vee q $ & material implication \\
$ [\neg p \vee \neg (\neg p \vee q)] \vee q $ & demorgans \\
$ [\neg p \vee  (\neg \neg p \wedge \neg q)] \vee q $ & demorgans \\
$ [\neg p \vee  (p \wedge \neg q)] \vee q $ & double negation \\
$ [(\neg p \vee p) \wedge(\neg p \vee \neg q)] \vee q $ & distributive \\
$ [(T) \wedge(\neg p \vee \neg q)] \vee q $ & negation law \\
$ [(\neg p \vee \neg q) \wedge T] \vee q $ & commutative \\
$ [\neg p \vee \neg q] \vee q $ & identity \\
$ \neg p \vee [\neg q \vee q]$ & associative \\
$ \neg p \vee T $ & negation law \\
$ T $ & domination \\ \hline
\end{tabular}
\newline \newline
LADBAP - This thing even looks a little like an arrow looking down. That is how BA this P is. True means that this is a tautology
 \newline \newline
$[(p \vee q) \wedge (p \rightarrow r) \wedge (q \rightarrow r)] \rightarrow r$\newline
\begin{tabular}{|c c|}\hline
$[(p \vee q) \wedge (p \rightarrow r) \wedge (q \rightarrow r)] \rightarrow r$ & given \\
$[(p \vee q) \wedge (\neg p \vee r) \wedge (q \rightarrow r)] \rightarrow r$ & material implication \\
$[(p \vee q) \wedge (\neg p \vee r) \wedge (\neg q \vee r)] \rightarrow r$ & material implication \\
$\neg [(p \vee q) \wedge (\neg p \vee r) \wedge (\neg q \vee r)] \vee r$ & material implication \\
$[\neg (p \vee q) \vee \neg (\neg p \vee r) \vee \neg (\neg q \vee r)] \vee r$ & demorgans \\
$[ (\neg p \wedge \neg q) \vee  (\neg\neg p \wedge \neg r) \vee \neg (\neg q \vee r)] \vee r$ & demorgans \\
$[ (\neg p \wedge \neg q) \vee  (\neg\neg p \wedge \neg r) \vee  (\neg \neg q \wedge \neg r)] \vee r$ & demorgans \\
$[ (\neg p \wedge \neg q) \vee  (p \wedge \neg r) \vee  (\neg \neg q \wedge \neg r)] \vee r$ & double negation \\
$[ (\neg p \wedge \neg q) \vee  (p \wedge \neg r) \vee  (q \wedge \neg r)] \vee r$ & double negation \\
$[ (\neg p \wedge \neg q) \vee  (\neg r \wedge p) \vee  (q \wedge \neg r)] \vee r$ & commutative \\
$ [(\neg p \wedge \neg q) \vee  (\neg r \wedge p) \vee  (\neg r \wedge q) ]\vee r$ & commutative \\
$ [(\neg p \wedge \neg q) \vee  (\neg r \wedge(p \vee q))] \vee r$ & distributive \\
$ r \vee [(\neg p \wedge \neg q) \vee (\neg r \wedge(p \vee q))]$ & commutative \\
$ [r \vee (\neg p \wedge \neg q)] \vee (\neg r \wedge(p \vee q))$ & associative \\
$ [r \vee (\neg p \wedge \neg q)] \vee \neg [r \vee \neg(p \vee q)]$ & demorgans  \\
$ [r \vee (\neg p \wedge \neg q)] \vee \neg[ r \vee (\neg p \wedge \neg q)]$ & demorgans \\
$ T $ & negation law \\\hline
\end{tabular}\newline
LADBAP - in the second to last line the things  in the brackets were the same. This allowed me to get a true using the negation law which means that the statement is tautologous.

\section*{1.3 \#14}
prove that $(\neg p \wedge (p \rightarrow q)) \rightarrow \neg q$ is a tautology \newline
\begin{tabular}{|c c|}\hline
$(\neg p \wedge (p \rightarrow q)) \rightarrow \neg q$ & given \\
$(\neg p \wedge (\neg p \vee q)) \rightarrow \neg q$ & material implication \\
$\neg (\neg p \wedge (\neg p \vee q)) \vee \neg q$ & material implication \\
$ (\neg \neg p \vee \neg (\neg p \vee q)) \vee \neg q$ & demorgans \\
$ (\neg \neg p \vee  (\neg \neg p \wedge q)) \vee \neg q$ & demorgans \\
$ ( p \vee  (\neg \neg p \wedge q)) \vee \neg q$ & double negation \\
$ ( p \vee  (p \wedge q)) \vee \neg q$ & double negation \\
$ ( (p \vee p) \wedge (p \vee q)) \vee \neg q$ & distributive \\
$ ( (T) \wedge (p \vee q)) \vee \neg q$ & idempotent \\
$ ( (p \vee q) \wedge T) \vee \neg q$ & commutative \\
$ ( p \vee q) \vee \neg q$ & identity \\
$  p \vee (q \vee \neg q)$ & associative \\
$  p \vee T$ & negation \\
$  T $ & domination \\ \hline
\end{tabular}
\newline
LADBAP - ended up with true so tautology

\section*{1.3 \#22}
show that $(p \rightarrow q) \wedge (p \rightarrow r)$ and $p \rightarrow (q \wedge r)$ are logically equivalent \newline
\begin{tabular}{|c c|}\hline
$(p \rightarrow q) \wedge (p \rightarrow r)$ & given\\
$(\neg p \vee q) \wedge (p \rightarrow r)$ & material implication\\
$(\neg p \vee q) \wedge (\neg p \vee r)$ & material implication\\
$\neg p \vee (q \wedge r)$ & distributive\\
$p \rightarrow (q \wedge r)$ & material implication\\ \hline
\end{tabular}
\newline
LADBAP - the last statement matches the second statement in the question exactly so the two statements are logically equivalent

\section*{1.4 \#6}
Let N(x) be the statement â€œx has visited North Dakota,â€ where the domain consists of the students in your school.\newline
a. There exists a student who has visited North Carolina\newline
b. Every student has visited North Carolina.\newline
e. Not all students have visited North Carolina\newline
f. Every student has not visited North Carolina\newline

\section*{1.4 \#10}
\begin{enumerate}
\item[a.] $\exists x(C(x) \wedge D(x) \wedge F(x))$
\item[b.] $\forall x(C(x) \vee D(x) \vee F(x))$
\item[c.] $\exists x(C(x) \wedge \neg D(x) \wedge F(x))$
\item[d.] $\forall x \neg (C(x) \wedge D(x) \wedge F(x))$
\item[e.] $\exists xC(x) \wedge \exists xD(x) \wedge \exists xF(x)$
\end{enumerate}

\section*{1.4 \#32}
\begin{enumerate}
\item[a.] $\forall d F(d)$ d $\in $ all dogs and F(d): d has fleas\newline
$\neg (\forall d F(d))$\newline
$\exists d \neg F(d)$ using demorgans\newline
There exists a dog that does not have fleas
\item[b.] $\exists h A(h)$ h $\in$ all horses and A(h): h can add\newline
$\neg (\exists h A(h))$\newline
$\forall h \neg A(h)$ using demorgans\newline
All horses can not add
\item[d.] $\forall m \neg F(m)$ m $\in$ monkeys and F(m): m can speak French  \newline
$\neg (\forall m \neg F(m))$\newline
$\exists m \neg \neg F(m))$ using demorgans\newline
$\exists m F(m))$ using double negation\newline
There exists a monkey that can speak french
\end{enumerate}

\section*{1.4 \#62}
a. $\forall x ( P(x) \rightarrow \neg S(x))$\newline
b. $\forall x ( R(x) \rightarrow S(x))$ \newline
c. $\forall x ( Q(x) \rightarrow P(x))$ \newline
d. $\forall x ( Q(x) \rightarrow \neg R(x))$ \newline
e.
\newline
$\neg P \vee \neg S$ - material implication from a \newline
$\neg R \vee S$ - material implication from b \newline
$\neg Q \vee P$ - material implication from c \newline
$\neg P \vee \neg R$ - 1 and 2 resolution\newline
$\neg Q \vee \neg R$ - 3 and 4 resolution
\newline \newline
it matches the material implcation from d - ( $\neg Q \vee \neg R$ )
so it is a correct conclusion
\end{document}
